Split code into spec and impl parts.

src/phase0/phase0_fork_choice_spec.dfy
@@ -10,86 +10,37 @@ import opened SimpleTypes
 import opened Entities
 import opened Consts
 
+/*
+    Return the epoch number at ``slot``.
+    */
+function method compute_epoch_at_slot(slot: Slot): Epoch
+requires valid_constants()
+{
+  Epoch_new(slot / SLOTS_PER_EPOCH)
+}
+
+/*
+    Return the start slot of ``epoch``.
+    */
+function method compute_start_slot_at_epoch(epoch: Epoch): Slot
+{
+  Slot_new(epoch * SLOTS_PER_EPOCH)
+}
+
 function method get_current_epoch(state: BeaconState): Epoch
 function method is_slashable_attestation_data(data1: AttestationData, data2: AttestationData): bool
 function method is_valid_indexed_attestation(state: BeaconState, attestation: IndexedAttestation): bool
 function method get_indexed_attestation(state: BeaconState, attestation: Attestation): IndexedAttestation
 function method get_active_validator_indices(state: BeaconState, epoch: Epoch): seq<ValidatorIndex>
 function method get_total_active_balance(state: BeaconState): Gwei
-method process_slots(state: BeaconState, slot: Slot) returns (status_: Outcome<BeaconState>)
-ensures process_slots_pure(state, slot) == status_
 function method process_slots_pure(state: BeaconState, slot: Slot): Outcome<BeaconState>
-method state_transition(state: BeaconState, block: SignedBeaconBlock, check: bool)
-returns (status_: Outcome<BeaconState>)
-ensures state_transition_pure(state, block, check) == status_
 function method state_transition_pure(state: BeaconState, block: SignedBeaconBlock, check: bool): Outcome<BeaconState>
-
-/*
-    Return the epoch number at ``slot``.
-    */
-function compute_epoch_at_slot(slot: Slot): Epoch
-requires valid_constants()
-{
-  Epoch_new(slot / SLOTS_PER_EPOCH)
-} by method {
-  return Epoch_new(slot / SLOTS_PER_EPOCH);
-}
-
-/*
-    Return the start slot of ``epoch``.
-    */
-function compute_start_slot_at_epoch(epoch: Epoch): Slot
-{
-  Slot_new(epoch * SLOTS_PER_EPOCH)
-} by method {
-  return Slot_new(epoch * SLOTS_PER_EPOCH);
-}
-
-method get_forkchoice_store(anchor_state: BeaconState, anchor_block: BeaconBlock)
-returns (status_: Outcome<Store>)
-{
-  var _ :- pyassert(anchor_block.state_root == hash_tree_root(anchor_state));
-  var anchor_root: Root := Root_new(hash_tree_root(anchor_block));
-  var anchor_epoch: Epoch := get_current_epoch(anchor_state);
-  var justified_checkpoint: Checkpoint := Checkpoint(anchor_epoch, anchor_root);
-  var finalized_checkpoint: Checkpoint := Checkpoint(anchor_epoch, anchor_root);
-  var proposer_boost_root: Root := Root_new(0);
-  var tmp_0 := Set_new({});
-  var tmp_1: Dict<Root, BeaconBlock> := Dict_new(map[anchor_root := anchor_block.copy()]);
-  var tmp_2: Dict<Root, BeaconState> := Dict_new(map[anchor_root := anchor_state.copy()]);
-  var tmp_3: Dict<Checkpoint, BeaconState> := Dict_new(map[justified_checkpoint := anchor_state.copy()]);
-  var tmp_4 := Dict_new(map[]);
-  var tmp_5 := new Store.Init(uint64_new(anchor_state.genesis_time + (SECONDS_PER_SLOT * anchor_state.slot)), anchor_state.genesis_time, justified_checkpoint, finalized_checkpoint, justified_checkpoint, proposer_boost_root, tmp_0, tmp_1, tmp_2, tmp_3, tmp_4);
-  return Result(tmp_5);
-}
-
-// imperative impure <==> functional impure <==> functional pure
-function get_slots_since_genesis(store: Store): (ret: int)
-reads store
-requires valid_time_slots(store) && valid_constants()
-ensures get_slots_since_genesis_pure(store.toPure()) == ret
-{
-  (store.time - store.genesis_time) / SECONDS_PER_SLOT
-} by method {
-  return (store.time - store.genesis_time) / SECONDS_PER_SLOT;
-}
 
 // functional pure
 function get_slots_since_genesis_pure(store: Store_dt): int
 requires valid_time_slots_pure(store) && valid_constants()
 {
   (store.time - store.genesis_time) / SECONDS_PER_SLOT
-}
-
-// imperative impure <==> functional impure <==> functional pure
-function get_current_slot(store: Store): (ret: Slot)
-reads store
-requires valid_time_slots(store) && valid_constants()
-ensures get_current_slot_pure(store.toPure()) == ret
-{
-  Slot_new(GENESIS_SLOT + get_slots_since_genesis(store))
-} by method {
-  return Slot_new(GENESIS_SLOT + get_slots_since_genesis(store));
 }
 
 // functional pure <==> functional impure
@@ -99,40 +50,10 @@ requires valid_time_slots_pure(store) && valid_constants()
   Slot_new(GENESIS_SLOT + get_slots_since_genesis_pure(store))
 }
 
-function compute_slots_since_epoch_start(slot: Slot): int
+function compute_slots_since_epoch_start_pure(slot: Slot): int
 requires valid_constants()
 {
-  slot - compute_start_slot_at_epoch(compute_epoch_at_slot(slot))
-} by method {
-  return slot - compute_start_slot_at_epoch(compute_epoch_at_slot(slot));
-}
-
-function get_ancestor(store: Store, root: Root, slot: Slot): (ret: Outcome<Root>)
-reads store, store.blocks
-requires valid_blocks(store.blocks)
-ensures get_ancestor_pure(store.toPure(), root, slot) == ret
-decreases if !store.blocks.contains(root) then 0 else store.blocks.get_nf(root).slot
-{
-  assert store.toPure().blocks == store.blocks.repr;
-  var block: BeaconBlock :- store.blocks.get(root);
-  if block.slot > slot then
-    get_ancestor(store, block.parent_root, slot)
-  else
-    if block.slot == slot then
-      Result(root)
-    else
-      Result(root)
-} by method {
-  var block: BeaconBlock :- store.blocks.get(root);
-  if block.slot > slot {
-    return get_ancestor(store, block.parent_root, slot);
-  } else {
-    if block.slot == slot {
-      return Result(root);
-    } else {
-      return Result(root);
-    }
-  }
+    slot - compute_start_slot_at_epoch(compute_epoch_at_slot(slot))
 }
 
 function get_ancestor_pure(store: Store_dt, root: Root, slot: Slot): (ret: Outcome<Root>)
@@ -148,193 +69,11 @@ decreases if root !in store.blocks then 0 else store.blocks[root].slot
     Result(root)
 }
 
-function get_latest_attesting_balance(store: Store, root: Root): Outcome<Gwei>
-reads store, store.blocks, store.checkpoint_states
-requires valid_constants()
-requires valid_blocks(store.blocks)
-{
-  var state: BeaconState :- store.checkpoint_states.get(store.justified_checkpoint);
-  var active_indices: seq<ValidatorIndex> := get_active_validator_indices(state, get_current_epoch(state));
-  var tmp_0 :- seq_filter_hf((i)
-     reads store, store.latest_messages, store.equivocating_indices, store.blocks
-     requires valid_blocks(store.blocks)
-   =>
-      if store.latest_messages.contains(i) && !store.equivocating_indices.contains(i) then
-        var tmp_0 :- store.latest_messages.get(i);
-        var tmp_1 :- store.blocks.get(root);
-        var tmp_2 :- get_ancestor(store, tmp_0.root, tmp_1.slot);
-        Result(tmp_2 == root)
-      else Result(false),
-    active_indices);
-  var tmp_1 :- seq_map_f((i) => var tmp_0 :- seq_get(state.validators, i); Result(tmp_0.effective_balance), tmp_0);
-  var attestation_score: Gwei := Gwei_new(seq_sum(tmp_1));
-  if store.proposer_boost_root == Root_new(0) then
-    Result(attestation_score)
-  else
-    var proposer_score: Gwei := Gwei_new(0);
-    var tmp_2 :- store.blocks.get(root);
-    var tmp_3 :- get_ancestor(store, store.proposer_boost_root, tmp_2.slot);
-    var proposer_score_2: Gwei :-
-      if tmp_3 == root then
-        var num_validators: int := |get_active_validator_indices(state, get_current_epoch(state))|;
-        var _ :- if num_validators == 0 then Exception else Result(());
-        var avg_balance: Gwei := get_total_active_balance(state) / num_validators;
-        var committee_size: uint64 := num_validators / SLOTS_PER_EPOCH;
-        var committee_weight: Gwei := committee_size * avg_balance;
-        var proposer_score_1: Gwei := committee_weight * PROPOSER_SCORE_BOOST / 100;
-        Result(proposer_score_1)
-      else
-        Result(proposer_score);
-    Result(attestation_score + proposer_score_2)
-} by method {
-  var state: BeaconState :- store.checkpoint_states.get(store.justified_checkpoint);
-  var active_indices: seq<ValidatorIndex> := get_active_validator_indices(state, get_current_epoch(state));
-  var tmp_0 :- seq_filter_hf((i)
-     reads store, store.latest_messages, store.equivocating_indices, store.blocks
-     requires valid_blocks(store.blocks)
-   =>
-      if store.latest_messages.contains(i) && !store.equivocating_indices.contains(i) then
-        var tmp_0 :- store.latest_messages.get(i);
-        var tmp_1 :- store.blocks.get(root);
-        var tmp_2 :- get_ancestor(store, tmp_0.root, tmp_1.slot);
-        Result(tmp_2 == root)
-      else Result(false),
-    active_indices);
-  var tmp_1 :- seq_map_f((i) => var tmp_0 :- seq_get(state.validators, i); Result(tmp_0.effective_balance), tmp_0);
-  var attestation_score: Gwei := Gwei_new(seq_sum(tmp_1));
-  if store.proposer_boost_root == Root_new(0) {
-    return Result(attestation_score);
-  }
-  var proposer_score: Gwei := Gwei_new(0);
-  var tmp_2 :- store.blocks.get(root);
-  var tmp_3 :- get_ancestor(store, store.proposer_boost_root, tmp_2.slot);
-  var proposer_score_2: Gwei :-
-    if tmp_3 == root then
-      var num_validators: int := |get_active_validator_indices(state, get_current_epoch(state))|;
-      var _ :- if num_validators == 0 then Exception else Result(());
-      var avg_balance: Gwei := get_total_active_balance(state) / num_validators;
-      var committee_size: uint64 := num_validators / SLOTS_PER_EPOCH;
-      var committee_weight: Gwei := committee_size * avg_balance;
-      var proposer_score_1: Gwei := committee_weight * PROPOSER_SCORE_BOOST / 100;
-      Result(proposer_score_1)
-    else
-      Result(proposer_score);
-  return Result(attestation_score + proposer_score_2);
-}
-
-method filter_block_tree(store: Store, block_root: Root, blocks: Dict<Root,BeaconBlock>)
-returns (status_: Outcome<bool>) 
-modifies blocks
-{
-  var block: BeaconBlock :- store.blocks.get(block_root);
-  var tmp_0 := store.blocks.keys();
-  var tmp_1 :- set_filter_hf((root) reads store, store.blocks => var tmp_0 :- store.blocks.get(root); Result(tmp_0.parent_root == block_root), tmp_0);
-  var children: seq<Root> := set_to_seq(tmp_1);
-  if seq_any(children) {
-    var tmp_0 := children;
-    var tmp_1 := PyList_new([]);
-    while tmp_0 != [] decreases tmp_0 {
-      var child := tmp_0[0];
-      tmp_0 := tmp_0[1..];
-      var tmp_2 :- filter_block_tree(store, child, blocks);
-      tmp_1.append(tmp_2);
-    }
-    var filter_block_tree_result: PyList<bool> := pylist(tmp_1);
-    if any(filter_block_tree_result) {
-      blocks.set_value(block_root, block);
-      return Result(true);
-    }
-    return Result(false);
-  }
-  var head_state: BeaconState :- store.block_states.get(block_root);
-  var correct_justified: bool := store.justified_checkpoint.epoch == GENESIS_EPOCH || head_state.current_justified_checkpoint == store.justified_checkpoint;
-  var correct_finalized: bool := store.finalized_checkpoint.epoch == GENESIS_EPOCH || head_state.finalized_checkpoint == store.finalized_checkpoint;
-  if correct_justified && correct_finalized {
-    blocks.set_value(block_root, block);
-    return Result(true);
-  }
-  return Result(false);
-}
-
-/*
-    Retrieve a filtered block tree from ``store``, only returning branches
-    whose leaf state's justified/finalized info agrees with that in ``store``.
-    */
-method get_filtered_block_tree(store: Store)
-returns (status_: Outcome<Dict<Root,BeaconBlock>>) 
-{
-  var base: Root := store.justified_checkpoint.root;
-  var blocks: Dict<Root,BeaconBlock> := Dict_new(map[]);
-  var _ := filter_block_tree(store, base, blocks);
-  return Result(blocks);
-}
-
-method get_head(store: Store)
-returns (status_: Outcome<Root>) 
-requires valid_constants()
-requires valid_blocks(store.blocks)
-decreases *
-{
-  var blocks: Dict<Root,BeaconBlock> :- get_filtered_block_tree(store);
-  var head: Root := store.justified_checkpoint.root;
-  var head_2 := head;
-  while true decreases * {
-    var tmp_0 := Set_new(blocks.keys());
-    var tmp_1 :- filter_f((root) reads blocks => var tmp_0 :- blocks.get(root); Result(tmp_0.parent_root == head_2), tmp_0);
-    var children: PyList<Root> := pylist(tmp_1);
-    if len(children) == 0 {
-      return Result(head_2);
-    }
-    var head_1: Root :- max_hf(children,
-      (root: Root)
-        reads store, store.blocks, store.checkpoint_states
-        requires valid_blocks(store.blocks)
-      => var tmp_0 :- get_latest_attesting_balance(store, root); Result((tmp_0, root)));
-    head_2 := head_1;
-  }
-}
-
-/*
-    To address the bouncing attack, only update conflicting justified
-    checkpoints in the fork choice if in the early slots of the epoch.
-    Otherwise, delay incorporation of new justified checkpoint until next epoch boundary.
-
-    See https://ethresear.ch/t/prevention-of-bouncing-attack-on-ffg/6114 for more detailed analysis and discussion.
-    */
-function should_update_justified_checkpoint(store: Store, new_justified_checkpoint: Checkpoint): (ret: Outcome<bool>)
-reads store, store.blocks
-requires valid_time_slots(store) && valid_constants()
-requires valid_blocks(store.blocks)
-ensures should_update_justified_checkpoint_pure(store.toPure(), new_justified_checkpoint)
-        == ret
-{
-  if compute_slots_since_epoch_start(get_current_slot(store)) < SAFE_SLOTS_TO_UPDATE_JUSTIFIED then
-    Result(true)
-  else
-    var justified_slot: Slot := compute_start_slot_at_epoch(store.justified_checkpoint.epoch);
-    var tmp_0 :- get_ancestor(store, new_justified_checkpoint.root, justified_slot);
-    if !(tmp_0 == store.justified_checkpoint.root) then
-      Result(false)
-    else
-      Result(true)
-} by method {
-  if compute_slots_since_epoch_start(get_current_slot(store)) < SAFE_SLOTS_TO_UPDATE_JUSTIFIED {
-    return Result(true);
-  }
-  var justified_slot: Slot := compute_start_slot_at_epoch(store.justified_checkpoint.epoch);
-  var tmp_0 :- get_ancestor(store, new_justified_checkpoint.root, justified_slot);
-  if !(tmp_0 == store.justified_checkpoint.root) {
-    return Result(false);
-  } else {
-    return Result(true);
-  }
-}
-
 function should_update_justified_checkpoint_pure(store: Store_dt, new_justified_checkpoint: Checkpoint): Outcome<bool>
 requires valid_time_slots_pure(store) && valid_constants()
 requires valid_blocks_pure(store.blocks)
 {
-  if compute_slots_since_epoch_start(get_current_slot_pure(store)) < SAFE_SLOTS_TO_UPDATE_JUSTIFIED then
+  if compute_slots_since_epoch_start_pure(get_current_slot_pure(store)) < SAFE_SLOTS_TO_UPDATE_JUSTIFIED then
     Result(true)
   else
     var justified_slot: Slot := compute_start_slot_at_epoch(store.justified_checkpoint.epoch);
@@ -343,28 +82,6 @@ requires valid_blocks_pure(store.blocks)
       Result(false)
     else
       Result(true)
-}
-
-
-function validate_target_epoch_against_current_time(store: Store, attestation: Attestation): (ret: Outcome<()>)
-reads store
-requires valid_constants()
-requires valid_time_slots(store)
-ensures validate_target_epoch_against_current_time_pure(store.toPure(), attestation)
-        == ret
-{
-  var target: Checkpoint := attestation.data.target;
-  var current_epoch: Epoch := compute_epoch_at_slot(get_current_slot(store));
-  var previous_epoch: Epoch := if (current_epoch > GENESIS_EPOCH) then current_epoch - 1 else GENESIS_EPOCH;
-  var _ :- pyassert(target.epoch in [current_epoch, previous_epoch]);
-  Result(())
-} by method {
-  var target: Checkpoint := attestation.data.target;
-  var current_epoch: Epoch := compute_epoch_at_slot(get_current_slot(store));
-  var previous_epoch: Epoch := if (current_epoch > GENESIS_EPOCH) then current_epoch - 1 else GENESIS_EPOCH;
-  var tmp_0 := PyList_new([current_epoch, previous_epoch]);
-  var _ :- pyassert(tmp_0.contains(target.epoch));
-  return Result(());
 }
 
 function validate_target_epoch_against_current_time_pure(store: Store_dt, attestation: Attestation): Outcome<()>
@@ -376,44 +93,6 @@ requires valid_time_slots_pure(store)
   var previous_epoch: Epoch := if (current_epoch > GENESIS_EPOCH) then current_epoch - 1 else GENESIS_EPOCH;
   var _ :- pyassert(target.epoch in [current_epoch, previous_epoch]);
   Result(())
-}
-
-function validate_on_attestation(store: Store, attestation: Attestation, is_from_block: bool): (ret: Outcome<()>)
-reads store, store.blocks
-requires valid_constants()
-requires valid_time_slots(store)
-requires valid_blocks(store.blocks)
-ensures validate_on_attestation_pure(store.toPure(), attestation, is_from_block)
-        == ret
-{
-  var target: Checkpoint := attestation.data.target;
-  var _ :- if !is_from_block then
-    validate_target_epoch_against_current_time(store, attestation)
-  else
-    Result(());
-  var _ :- pyassert(target.epoch == compute_epoch_at_slot(attestation.data.slot));
-  var _ :- pyassert(store.blocks.contains(target.root));
-  var _ :- pyassert(store.blocks.contains(attestation.data.beacon_block_root));
-  var _ :- pyassert(store.blocks.get_nf(attestation.data.beacon_block_root).slot <= attestation.data.slot);
-  var target_slot: Slot := compute_start_slot_at_epoch(target.epoch);
-  var tmp_0 :- get_ancestor(store, attestation.data.beacon_block_root, target_slot);
-  var _ :- pyassert(target.root == tmp_0);
-  var _ :- pyassert(get_current_slot(store) >= (attestation.data.slot + 1));
-  Result(())
-} by method {
-  var target: Checkpoint := attestation.data.target;
-  if !is_from_block {
-    var _ :- validate_target_epoch_against_current_time(store, attestation);
-  }
-  var _ :- pyassert(target.epoch == compute_epoch_at_slot(attestation.data.slot));
-  var _ :- pyassert(store.blocks.contains(target.root));
-  var _ :- pyassert(store.blocks.contains(attestation.data.beacon_block_root));
-  var _ :- pyassert(store.blocks.get_nf(attestation.data.beacon_block_root).slot <= attestation.data.slot);
-  var target_slot: Slot := compute_start_slot_at_epoch(target.epoch);
-  var tmp_0 :- get_ancestor(store, attestation.data.beacon_block_root, target_slot);
-  var _ :- pyassert(target.root == tmp_0);
-  var _ :- pyassert(get_current_slot(store) >= (attestation.data.slot + 1));
-  return Result(());
 }
 
 function validate_on_attestation_pure(store: Store_dt, attestation: Attestation, is_from_block: bool): Outcome<()>
@@ -437,25 +116,6 @@ requires valid_blocks_pure(store.blocks)
   Result(())
 }
 
-method store_target_checkpoint_state(store: Store, target: Checkpoint)
-returns (status_: Outcome<()>) 
-modifies store.checkpoint_states
-ensures var pure_ret := store_target_checkpoint_state_pure(old(store.toPure()), target);
-        && !status_.IsFailure() <==> !pure_ret.IsFailure()
-        && !status_.IsFailure() ==> store.toPure() == pure_ret.Extract()
-{
-  assert store.toPure().blocks == store.blocks.repr;
-  status_ := Result(());
-  if !store.checkpoint_states.contains(target) {
-    var tmp_0 :- store.block_states.get(target.root);
-    var base_state: BeaconState := tmp_0.copy();
-    if base_state.slot < compute_start_slot_at_epoch(target.epoch) {
-      base_state :- process_slots(base_state, compute_start_slot_at_epoch(target.epoch));
-    }
-    store.checkpoint_states.set_value(target, base_state);
-  }
-}
-
 function store_target_checkpoint_state_pure(store: Store_dt, target: Checkpoint): Outcome<Store_dt>
 {
   if target !in store.checkpoint_states then
@@ -470,49 +130,6 @@ function store_target_checkpoint_state_pure(store: Store_dt, target: Checkpoint)
     Result(store)
   else
     Result(store)
-} by method {
-  var store := store;
-  if target !in store.checkpoint_states {
-    var tmp_0 :- map_get(store.block_states, target.root);
-    var base_state: BeaconState := tmp_0.copy();
-    if base_state.slot < compute_start_slot_at_epoch(target.epoch) {
-      base_state :- process_slots(base_state, compute_start_slot_at_epoch(target.epoch));
-    }
-    store := store.(checkpoint_states := store.checkpoint_states[target := base_state]);
-  }
-  return Result(store);
-}
-
-
-method update_latest_messages(store: Store, attesting_indices: seq<ValidatorIndex>, attestation: Attestation)
-modifies store.latest_messages
-ensures store.toPure() == update_latest_messages_pure(old(store.toPure()), attesting_indices, attestation)
-{
-  var target: Checkpoint := attestation.data.target;
-  var beacon_block_root: Root := attestation.data.beacon_block_root;
-  var non_equivocating_attesting_indices: seq<ValidatorIndex> := seq_filter_h((i) reads store, store.equivocating_indices => !store.equivocating_indices.contains(i), attesting_indices);
-  var tmp := store.equivocating_indices.repr;
-  assume non_equivocating_attesting_indices == seq_filter((i) => i !in tmp, attesting_indices);
-  var tmp_for_0: seq<ValidatorIndex> := non_equivocating_attesting_indices;
-  
-  ghost var processed: seq<ValidatorIndex> := [];
-  ghost var loop_body := (store: Store_dt, i: ValidatorIndex) =>
-    if i !in store.latest_messages || target.epoch > store.latest_messages[i].epoch then
-      store.(latest_messages := store.latest_messages[i := LatestMessage(target.epoch, beacon_block_root)])
-    else
-      store;
-  while tmp_for_0 != [] decreases tmp_for_0
-  invariant processed + tmp_for_0 == non_equivocating_attesting_indices
-  invariant seq_loop(processed, old(store.toPure()), loop_body) == store.toPure()
-  {
-    var i: ValidatorIndex := tmp_for_0[0];
-    tmp_for_0 := tmp_for_0[1..];
-    if !store.latest_messages.contains(i) || target.epoch > store.latest_messages.get_nf(i).epoch {
-      store.latest_messages.set_value(i, LatestMessage(target.epoch, beacon_block_root));
-    }
-    processed := processed + [i];
-  }
-  assert processed == non_equivocating_attesting_indices;
 }
 
 function update_latest_messages_pure(store: Store_dt, attesting_indices: seq<ValidatorIndex>, attestation: Attestation): Store_dt
@@ -529,35 +146,6 @@ function update_latest_messages_pure(store: Store_dt, attesting_indices: seq<Val
   store
 }
 
-method on_tick(store: Store, time: uint64)
-returns (status_: Outcome<()>) 
-requires time >= store.time
-requires valid_constants()
-requires valid_time_slots(store)
-requires valid_blocks(store.blocks)
-modifies store
-ensures !status_.IsFailure() <==> !on_tick_pure(old(store.toPure()), time).IsFailure()
-ensures !status_.IsFailure() ==> store.toPure() == on_tick_pure(old(store.toPure()), time).Extract()
-{
-  status_ := Result(());
-  var previous_slot: Slot := get_current_slot(store);
-  store.time := time;
-  var current_slot: Slot := get_current_slot(store);
-  if current_slot > previous_slot {
-    store.proposer_boost_root := Root_new(0);
-  }
-  if !(current_slot > previous_slot && compute_slots_since_epoch_start(current_slot) == 0) {
-    return;
-  }
-  if store.best_justified_checkpoint.epoch > store.justified_checkpoint.epoch {
-    var finalized_slot: Slot := compute_start_slot_at_epoch(store.finalized_checkpoint.epoch);
-    var ancestor_at_finalized_slot :- get_ancestor(store, store.best_justified_checkpoint.root, finalized_slot);
-    if ancestor_at_finalized_slot == store.finalized_checkpoint.root {
-      store.justified_checkpoint := store.best_justified_checkpoint;
-    }
-  }
-}
-
 function on_tick_pure(store: Store_dt, time: uint64): Outcome<Store_dt>
 requires time >= store.time
 requires valid_constants()
@@ -572,7 +160,7 @@ requires valid_blocks_pure(store.blocks)
     store
   else
     store;
-  if !(current_slot > previous_slot && compute_slots_since_epoch_start(current_slot) == 0) then
+  if !(current_slot > previous_slot && compute_slots_since_epoch_start_pure(current_slot) == 0) then
     Result(store)
   else
     if store.best_justified_checkpoint.epoch > store.justified_checkpoint.epoch then
@@ -586,51 +174,6 @@ requires valid_blocks_pure(store.blocks)
     else
       Result(store)
 } 
-
-method on_block(store: Store, signed_block: SignedBeaconBlock)
-returns (status_: Outcome<()>) 
-requires valid_constants()
-requires valid_time_slots(store)
-requires valid_blocks(store.blocks)
-modifies store, store.blocks, store.block_states
-ensures var pure_out := on_block_pure(old(store.toPure()), signed_block);
-        && !status_.IsFailure() <==> !pure_out.IsFailure()
-        && !status_.IsFailure() ==> store.toPure() == pure_out.Extract()
-{
-  status_ := Result(());
-  var block: BeaconBlock := signed_block.message;
-  var _ :- pyassert(store.block_states.contains(block.parent_root));
-  var tmp_0 :- store.block_states.get(block.parent_root);
-  var pre_state: BeaconState := tmp_0.copy();
-  var _ :- pyassert(get_current_slot(store) >= block.slot);
-  var finalized_slot: Slot := compute_start_slot_at_epoch(store.finalized_checkpoint.epoch);
-  var _ :- pyassert(block.slot > finalized_slot);
-  var tmp_1 :- get_ancestor(store, block.parent_root, finalized_slot);
-  var _ :- pyassert(tmp_1 == store.finalized_checkpoint.root);
-  var state: BeaconState := pre_state.copy();
-  state :- state_transition(state, signed_block, true);
-  store.blocks.set_value(hash_tree_root(block), block);
-  assume valid_blocks(store.blocks);
-  store.block_states.set_value(hash_tree_root(block), state);
-  var time_into_slot: uint64 := (store.time - store.genesis_time) % SECONDS_PER_SLOT;
-  var is_before_attesting_interval: bool := time_into_slot < (SECONDS_PER_SLOT / INTERVALS_PER_SLOT);
-  if get_current_slot(store) == block.slot && is_before_attesting_interval {
-    store.proposer_boost_root := Root_new(hash_tree_root(block));
-  }
-  if state.current_justified_checkpoint.epoch > store.justified_checkpoint.epoch {
-    if state.current_justified_checkpoint.epoch > store.best_justified_checkpoint.epoch {
-      store.best_justified_checkpoint := state.current_justified_checkpoint;
-    }
-    var tmp_2 :- should_update_justified_checkpoint(store, state.current_justified_checkpoint);
-    if tmp_2 {
-      store.justified_checkpoint := state.current_justified_checkpoint;
-    }
-  }
-  if state.finalized_checkpoint.epoch > store.finalized_checkpoint.epoch {
-    store.finalized_checkpoint := state.finalized_checkpoint;
-    store.justified_checkpoint := state.current_justified_checkpoint;
-  }
-}
 
 function on_block_pure(store: Store_dt, signed_block: SignedBeaconBlock): Outcome<Store_dt>
 requires valid_constants()
@@ -683,31 +226,6 @@ requires valid_blocks_pure(store.blocks)
   Result(store)
 } 
 
-/*
-    Run ``on_attestation`` upon receiving a new ``attestation`` from either within a block or directly on the wire.
-
-    An ``attestation`` that is asserted as invalid may be valid at a later time,
-    consider scheduling it for later processing in such case.
-    */
-method on_attestation(store: Store, attestation: Attestation, is_from_block: bool)
-returns (status_: Outcome<()>) 
-requires valid_constants()
-requires valid_time_slots(store)
-requires valid_blocks(store.blocks)
-modifies store.latest_messages, store.checkpoint_states
-ensures var pure_out := on_attestation_pure(old(store.toPure()), attestation, is_from_block);
-        && !status_.IsFailure() <==> !pure_out.IsFailure()
-        && !status_.IsFailure() ==> store.toPure() == pure_out.Extract()
-{
-  status_ := Result(());
-  var _ :- validate_on_attestation(store, attestation, is_from_block);
-  var _ :- store_target_checkpoint_state(store, attestation.data.target);
-  var target_state: BeaconState :- store.checkpoint_states.get(attestation.data.target);
-  var indexed_attestation: IndexedAttestation := get_indexed_attestation(target_state, attestation);
-  var _ :- pyassert(is_valid_indexed_attestation(target_state, indexed_attestation));
-  update_latest_messages(store, indexed_attestation.attesting_indices, attestation);
-}
-
 function on_attestation_pure(store: Store_dt, attestation: Attestation, is_from_block: bool): Outcome<Store_dt>
 requires valid_constants()
 requires valid_time_slots_pure(store)
@@ -715,42 +233,12 @@ requires valid_blocks_pure(store.blocks)
 {
   var _ :- validate_on_attestation_pure(store, attestation, is_from_block);
   var store :- store_target_checkpoint_state_pure(store, attestation.data.target);
-  var tmp := map_get(store.checkpoint_states, attestation.data.target);
-  if tmp.IsFailure() then
-    Exception
-  else
-  var target_state: BeaconState := tmp.Extract();
+  var target_state: BeaconState :- map_get(store.checkpoint_states, attestation.data.target);
   var indexed_attestation: IndexedAttestation := get_indexed_attestation(target_state, attestation);
   var _ :- pyassert(is_valid_indexed_attestation(target_state, indexed_attestation));
   var store := update_latest_messages_pure(store, indexed_attestation.attesting_indices, attestation);
   Result(store)
 } 
-
-/*
-    Run ``on_attester_slashing`` immediately upon receiving a new ``AttesterSlashing``
-    from either within a block or directly on the wire.
-    */
-method on_attester_slashing(store: Store, attester_slashing: AttesterSlashing)
-returns (status_: Outcome<()>) 
-modifies store.equivocating_indices
-{
-  status_ := Result(());
-  var attestation_1: IndexedAttestation := attester_slashing.attestation_1;
-  var attestation_2: IndexedAttestation := attester_slashing.attestation_2;
-  var _ :- pyassert(is_slashable_attestation_data(attestation_1.data, attestation_2.data));
-  var state: BeaconState :- store.block_states.get(store.justified_checkpoint.root);
-  var _ :- pyassert(is_valid_indexed_attestation(state, attestation_1));
-  var _ :- pyassert(is_valid_indexed_attestation(state, attestation_2));
-  var indices: set<ValidatorIndex> := seq_to_set(attestation_1.attesting_indices) * seq_to_set(attestation_2.attesting_indices);
-  var tmp_for_0: set<ValidatorIndex> := indices;
-  while tmp_for_0 != {} decreases tmp_for_0 {
-    var index: ValidatorIndex :| index in tmp_for_0;
-    tmp_for_0 := tmp_for_0 - {index};
-    store.equivocating_indices.add(index);
-  }
-}
-
-function method seq_intersection<T>(a: seq<T>, b: seq<T>): seq<T>
 
 function on_attester_slashing_pure(store: Store_dt, attester_slashing: AttesterSlashing): Outcome<Store_dt>
 {
@@ -765,20 +253,4 @@ function on_attester_slashing_pure(store: Store_dt, attester_slashing: AttesterS
     store.(equivocating_indices := store.equivocating_indices + {index});
   var store := set_loop(indices, store, loop_body);
   Result(store)
-} by method {
-  var store := store;
-  var attestation_1: IndexedAttestation := attester_slashing.attestation_1;
-  var attestation_2: IndexedAttestation := attester_slashing.attestation_2;
-  var _ :- pyassert(is_slashable_attestation_data(attestation_1.data, attestation_2.data));
-  var state: BeaconState :- map_get(store.block_states, store.justified_checkpoint.root);
-  var _ :- pyassert(is_valid_indexed_attestation(state, attestation_1));
-  var _ :- pyassert(is_valid_indexed_attestation(state, attestation_2));
-  var indices: set<ValidatorIndex> := seq_to_set(attestation_1.attesting_indices) * seq_to_set(attestation_2.attesting_indices);
-  var tmp_for_0: set<ValidatorIndex> := indices;
-  while tmp_for_0 != {} decreases tmp_for_0 {
-    var index: ValidatorIndex :| index in tmp_for_0;
-    tmp_for_0 := tmp_for_0 - {index};
-    store := store.(equivocating_indices := store.equivocating_indices + {index});
-  }
-  return Result(store);
 }
