src/phase0/phase0_fork_choice_impl.dfy
@@ -1,0 +1,511 @@
+include "ssz.dfy"
+include "simpletypes.dfy"
+include "entities.dfy"
+include "consts.dfy"
+
+include "helpers.dfy"
+include "phase0_fork_choice_spec.dfy"
+
+import opened SSZ
+import opened SimpleTypes
+import opened Entities
+import opened Consts
+
+
+method process_slots(state: BeaconState, slot: Slot) returns (status_: Outcome<BeaconState>)
+ensures process_slots_pure(state, slot) == status_
+
+method state_transition(state: BeaconState, block: SignedBeaconBlock, check: bool)
+returns (status_: Outcome<BeaconState>)
+ensures state_transition_pure(state, block, check) == status_
+
+
+method get_forkchoice_store(anchor_state: BeaconState, anchor_block: BeaconBlock)
+returns (status_: Outcome<Store>)
+{
+  var _ :- pyassert(anchor_block.state_root == hash_tree_root(anchor_state));
+  var anchor_root: Root := Root_new(hash_tree_root(anchor_block));
+  var anchor_epoch: Epoch := get_current_epoch(anchor_state);
+  var justified_checkpoint: Checkpoint := Checkpoint(anchor_epoch, anchor_root);
+  var finalized_checkpoint: Checkpoint := Checkpoint(anchor_epoch, anchor_root);
+  var proposer_boost_root: Root := Root_new(0);
+  var tmp_0 := Set_new({});
+  var tmp_1: Dict<Root, BeaconBlock> := Dict_new(map[anchor_root := anchor_block.copy()]);
+  var tmp_2: Dict<Root, BeaconState> := Dict_new(map[anchor_root := anchor_state.copy()]);
+  var tmp_3: Dict<Checkpoint, BeaconState> := Dict_new(map[justified_checkpoint := anchor_state.copy()]);
+  var tmp_4 := Dict_new(map[]);
+  var tmp_5 := new Store.Init(uint64_new(anchor_state.genesis_time + (SECONDS_PER_SLOT * anchor_state.slot)), anchor_state.genesis_time, justified_checkpoint, finalized_checkpoint, justified_checkpoint, proposer_boost_root, tmp_0, tmp_1, tmp_2, tmp_3, tmp_4);
+  return Result(tmp_5);
+}
+
+// imperative impure <==> functional impure <==> functional pure
+function get_slots_since_genesis(store: Store): (ret: int)
+reads store
+requires valid_time_slots(store) && valid_constants()
+ensures get_slots_since_genesis_pure(store.toPure()) == ret
+{
+  (store.time - store.genesis_time) / SECONDS_PER_SLOT
+} by method {
+  return (store.time - store.genesis_time) / SECONDS_PER_SLOT;
+}
+
+// imperative impure <==> functional impure <==> functional pure
+function get_current_slot(store: Store): (ret: Slot)
+reads store
+requires valid_time_slots(store) && valid_constants()
+ensures get_current_slot_pure(store.toPure()) == ret
+{
+  Slot_new(GENESIS_SLOT + get_slots_since_genesis(store))
+} by method {
+  return Slot_new(GENESIS_SLOT + get_slots_since_genesis(store));
+}
+
+function compute_slots_since_epoch_start(slot: Slot): int
+requires valid_constants()
+{
+  slot - compute_start_slot_at_epoch(compute_epoch_at_slot(slot))
+} by method {
+  return slot - compute_start_slot_at_epoch(compute_epoch_at_slot(slot));
+}
+
+function get_ancestor(store: Store, root: Root, slot: Slot): (ret: Outcome<Root>)
+reads store, store.blocks
+requires valid_blocks(store.blocks)
+ensures get_ancestor_pure(store.toPure(), root, slot) == ret
+decreases if !store.blocks.contains(root) then 0 else store.blocks.get_nf(root).slot
+{
+  assert store.toPure().blocks == store.blocks.repr;
+  var block: BeaconBlock :- store.blocks.get(root);
+  if block.slot > slot then
+    get_ancestor(store, block.parent_root, slot)
+  else
+    if block.slot == slot then
+      Result(root)
+    else
+      Result(root)
+} by method {
+  var block: BeaconBlock :- store.blocks.get(root);
+  if block.slot > slot {
+    return get_ancestor(store, block.parent_root, slot);
+  } else {
+    if block.slot == slot {
+      return Result(root);
+    } else {
+      return Result(root);
+    }
+  }
+}
+
+function get_latest_attesting_balance(store: Store, root: Root): Outcome<Gwei>
+reads store, store.blocks, store.checkpoint_states
+requires valid_constants()
+requires valid_blocks(store.blocks)
+{
+  var state: BeaconState :- store.checkpoint_states.get(store.justified_checkpoint);
+  var active_indices: seq<ValidatorIndex> := get_active_validator_indices(state, get_current_epoch(state));
+  var tmp_0 :- seq_filter_hf((i)
+     reads store, store.latest_messages, store.equivocating_indices, store.blocks
+     requires valid_blocks(store.blocks)
+   =>
+      if store.latest_messages.contains(i) && !store.equivocating_indices.contains(i) then
+        var tmp_0 :- store.latest_messages.get(i);
+        var tmp_1 :- store.blocks.get(root);
+        var tmp_2 :- get_ancestor(store, tmp_0.root, tmp_1.slot);
+        Result(tmp_2 == root)
+      else Result(false),
+    active_indices);
+  var tmp_1 :- seq_map_f((i) => var tmp_0 :- seq_get(state.validators, i); Result(tmp_0.effective_balance), tmp_0);
+  var attestation_score: Gwei := Gwei_new(seq_sum(tmp_1));
+  if store.proposer_boost_root == Root_new(0) then
+    Result(attestation_score)
+  else
+    var proposer_score: Gwei := Gwei_new(0);
+    var tmp_2 :- store.blocks.get(root);
+    var tmp_3 :- get_ancestor(store, store.proposer_boost_root, tmp_2.slot);
+    var proposer_score_2: Gwei :-
+      if tmp_3 == root then
+        var num_validators: int := |get_active_validator_indices(state, get_current_epoch(state))|;
+        var _ :- if num_validators == 0 then Exception else Result(());
+        var avg_balance: Gwei := get_total_active_balance(state) / num_validators;
+        var committee_size: uint64 := num_validators / SLOTS_PER_EPOCH;
+        var committee_weight: Gwei := committee_size * avg_balance;
+        var proposer_score_1: Gwei := committee_weight * PROPOSER_SCORE_BOOST / 100;
+        Result(proposer_score_1)
+      else
+        Result(proposer_score);
+    Result(attestation_score + proposer_score_2)
+} by method {
+  var state: BeaconState :- store.checkpoint_states.get(store.justified_checkpoint);
+  var active_indices: seq<ValidatorIndex> := get_active_validator_indices(state, get_current_epoch(state));
+  var tmp_0 :- seq_filter_hf((i)
+     reads store, store.latest_messages, store.equivocating_indices, store.blocks
+     requires valid_blocks(store.blocks)
+   =>
+      if store.latest_messages.contains(i) && !store.equivocating_indices.contains(i) then
+        var tmp_0 :- store.latest_messages.get(i);
+        var tmp_1 :- store.blocks.get(root);
+        var tmp_2 :- get_ancestor(store, tmp_0.root, tmp_1.slot);
+        Result(tmp_2 == root)
+      else Result(false),
+    active_indices);
+  var tmp_1 :- seq_map_f((i) => var tmp_0 :- seq_get(state.validators, i); Result(tmp_0.effective_balance), tmp_0);
+  var attestation_score: Gwei := Gwei_new(seq_sum(tmp_1));
+  if store.proposer_boost_root == Root_new(0) {
+    return Result(attestation_score);
+  }
+  var proposer_score: Gwei := Gwei_new(0);
+  var tmp_2 :- store.blocks.get(root);
+  var tmp_3 :- get_ancestor(store, store.proposer_boost_root, tmp_2.slot);
+  var proposer_score_2: Gwei :-
+    if tmp_3 == root then
+      var num_validators: int := |get_active_validator_indices(state, get_current_epoch(state))|;
+      var _ :- if num_validators == 0 then Exception else Result(());
+      var avg_balance: Gwei := get_total_active_balance(state) / num_validators;
+      var committee_size: uint64 := num_validators / SLOTS_PER_EPOCH;
+      var committee_weight: Gwei := committee_size * avg_balance;
+      var proposer_score_1: Gwei := committee_weight * PROPOSER_SCORE_BOOST / 100;
+      Result(proposer_score_1)
+    else
+      Result(proposer_score);
+  return Result(attestation_score + proposer_score_2);
+}
+
+method filter_block_tree(store: Store, block_root: Root, blocks: Dict<Root,BeaconBlock>)
+returns (status_: Outcome<bool>) 
+modifies blocks
+{
+  var block: BeaconBlock :- store.blocks.get(block_root);
+  var tmp_0 := store.blocks.keys();
+  var tmp_1 :- set_filter_hf((root) reads store, store.blocks => var tmp_0 :- store.blocks.get(root); Result(tmp_0.parent_root == block_root), tmp_0);
+  var children: seq<Root> := set_to_seq(tmp_1);
+  if seq_any(children) {
+    var tmp_0 := children;
+    var tmp_1 := PyList_new([]);
+    while tmp_0 != [] decreases tmp_0 {
+      var child := tmp_0[0];
+      tmp_0 := tmp_0[1..];
+      var tmp_2 :- filter_block_tree(store, child, blocks);
+      tmp_1.append(tmp_2);
+    }
+    var filter_block_tree_result: PyList<bool> := pylist(tmp_1);
+    if any(filter_block_tree_result) {
+      blocks.set_value(block_root, block);
+      return Result(true);
+    }
+    return Result(false);
+  }
+  var head_state: BeaconState :- store.block_states.get(block_root);
+  var correct_justified: bool := store.justified_checkpoint.epoch == GENESIS_EPOCH || head_state.current_justified_checkpoint == store.justified_checkpoint;
+  var correct_finalized: bool := store.finalized_checkpoint.epoch == GENESIS_EPOCH || head_state.finalized_checkpoint == store.finalized_checkpoint;
+  if correct_justified && correct_finalized {
+    blocks.set_value(block_root, block);
+    return Result(true);
+  }
+  return Result(false);
+}
+
+/*
+    Retrieve a filtered block tree from ``store``, only returning branches
+    whose leaf state's justified/finalized info agrees with that in ``store``.
+    */
+method get_filtered_block_tree(store: Store)
+returns (status_: Outcome<Dict<Root,BeaconBlock>>) 
+{
+  var base: Root := store.justified_checkpoint.root;
+  var blocks: Dict<Root,BeaconBlock> := Dict_new(map[]);
+  var _ := filter_block_tree(store, base, blocks);
+  return Result(blocks);
+}
+
+method get_head(store: Store)
+returns (status_: Outcome<Root>) 
+requires valid_constants()
+requires valid_blocks(store.blocks)
+decreases *
+{
+  var blocks: Dict<Root,BeaconBlock> :- get_filtered_block_tree(store);
+  var head: Root := store.justified_checkpoint.root;
+  var head_2 := head;
+  while true decreases * {
+    var tmp_0 := Set_new(blocks.keys());
+    var tmp_1 :- filter_f((root) reads blocks => var tmp_0 :- blocks.get(root); Result(tmp_0.parent_root == head_2), tmp_0);
+    var children: PyList<Root> := pylist(tmp_1);
+    if len(children) == 0 {
+      return Result(head_2);
+    }
+    var head_1: Root :- max_hf(children,
+      (root: Root)
+        reads store, store.blocks, store.checkpoint_states
+        requires valid_blocks(store.blocks)
+      => var tmp_0 :- get_latest_attesting_balance(store, root); Result((tmp_0, root)));
+    head_2 := head_1;
+  }
+}
+
+/*
+    To address the bouncing attack, only update conflicting justified
+    checkpoints in the fork choice if in the early slots of the epoch.
+    Otherwise, delay incorporation of new justified checkpoint until next epoch boundary.
+
+    See https://ethresear.ch/t/prevention-of-bouncing-attack-on-ffg/6114 for more detailed analysis and discussion.
+    */
+function should_update_justified_checkpoint(store: Store, new_justified_checkpoint: Checkpoint): (ret: Outcome<bool>)
+reads store, store.blocks
+requires valid_time_slots(store) && valid_constants()
+requires valid_blocks(store.blocks)
+ensures should_update_justified_checkpoint_pure(store.toPure(), new_justified_checkpoint)
+        == ret
+{
+  if compute_slots_since_epoch_start(get_current_slot(store)) < SAFE_SLOTS_TO_UPDATE_JUSTIFIED then
+    Result(true)
+  else
+    var justified_slot: Slot := compute_start_slot_at_epoch(store.justified_checkpoint.epoch);
+    var tmp_0 :- get_ancestor(store, new_justified_checkpoint.root, justified_slot);
+    if !(tmp_0 == store.justified_checkpoint.root) then
+      Result(false)
+    else
+      Result(true)
+} by method {
+  if compute_slots_since_epoch_start(get_current_slot(store)) < SAFE_SLOTS_TO_UPDATE_JUSTIFIED {
+    return Result(true);
+  }
+  var justified_slot: Slot := compute_start_slot_at_epoch(store.justified_checkpoint.epoch);
+  var tmp_0 :- get_ancestor(store, new_justified_checkpoint.root, justified_slot);
+  if !(tmp_0 == store.justified_checkpoint.root) {
+    return Result(false);
+  } else {
+    return Result(true);
+  }
+}
+
+function validate_target_epoch_against_current_time(store: Store, attestation: Attestation): (ret: Outcome<()>)
+reads store
+requires valid_constants()
+requires valid_time_slots(store)
+ensures validate_target_epoch_against_current_time_pure(store.toPure(), attestation)
+        == ret
+{
+  var target: Checkpoint := attestation.data.target;
+  var current_epoch: Epoch := compute_epoch_at_slot(get_current_slot(store));
+  var previous_epoch: Epoch := if (current_epoch > GENESIS_EPOCH) then current_epoch - 1 else GENESIS_EPOCH;
+  var _ :- pyassert(target.epoch in [current_epoch, previous_epoch]);
+  Result(())
+} by method {
+  var target: Checkpoint := attestation.data.target;
+  var current_epoch: Epoch := compute_epoch_at_slot(get_current_slot(store));
+  var previous_epoch: Epoch := if (current_epoch > GENESIS_EPOCH) then current_epoch - 1 else GENESIS_EPOCH;
+  var tmp_0 := PyList_new([current_epoch, previous_epoch]);
+  var _ :- pyassert(tmp_0.contains(target.epoch));
+  return Result(());
+}
+
+function validate_on_attestation(store: Store, attestation: Attestation, is_from_block: bool): (ret: Outcome<()>)
+reads store, store.blocks
+requires valid_constants()
+requires valid_time_slots(store)
+requires valid_blocks(store.blocks)
+ensures validate_on_attestation_pure(store.toPure(), attestation, is_from_block)
+        == ret
+{
+  var target: Checkpoint := attestation.data.target;
+  var _ :- if !is_from_block then
+    validate_target_epoch_against_current_time(store, attestation)
+  else
+    Result(());
+  var _ :- pyassert(target.epoch == compute_epoch_at_slot(attestation.data.slot));
+  var _ :- pyassert(store.blocks.contains(target.root));
+  var _ :- pyassert(store.blocks.contains(attestation.data.beacon_block_root));
+  var _ :- pyassert(store.blocks.get_nf(attestation.data.beacon_block_root).slot <= attestation.data.slot);
+  var target_slot: Slot := compute_start_slot_at_epoch(target.epoch);
+  var tmp_0 :- get_ancestor(store, attestation.data.beacon_block_root, target_slot);
+  var _ :- pyassert(target.root == tmp_0);
+  var _ :- pyassert(get_current_slot(store) >= (attestation.data.slot + 1));
+  Result(())
+} by method {
+  var target: Checkpoint := attestation.data.target;
+  if !is_from_block {
+    var _ :- validate_target_epoch_against_current_time(store, attestation);
+  }
+  var _ :- pyassert(target.epoch == compute_epoch_at_slot(attestation.data.slot));
+  var _ :- pyassert(store.blocks.contains(target.root));
+  var _ :- pyassert(store.blocks.contains(attestation.data.beacon_block_root));
+  var _ :- pyassert(store.blocks.get_nf(attestation.data.beacon_block_root).slot <= attestation.data.slot);
+  var target_slot: Slot := compute_start_slot_at_epoch(target.epoch);
+  var tmp_0 :- get_ancestor(store, attestation.data.beacon_block_root, target_slot);
+  var _ :- pyassert(target.root == tmp_0);
+  var _ :- pyassert(get_current_slot(store) >= (attestation.data.slot + 1));
+  return Result(());
+}
+
+method store_target_checkpoint_state(store: Store, target: Checkpoint)
+returns (status_: Outcome<()>) 
+modifies store.checkpoint_states
+ensures var pure_ret := store_target_checkpoint_state_pure(old(store.toPure()), target);
+        && !status_.IsFailure() <==> !pure_ret.IsFailure()
+        && !status_.IsFailure() ==> store.toPure() == pure_ret.Extract()
+{
+  assert store.toPure().blocks == store.blocks.repr;
+  status_ := Result(());
+  if !store.checkpoint_states.contains(target) {
+    var tmp_0 :- store.block_states.get(target.root);
+    var base_state: BeaconState := tmp_0.copy();
+    if base_state.slot < compute_start_slot_at_epoch(target.epoch) {
+      base_state :- process_slots(base_state, compute_start_slot_at_epoch(target.epoch));
+    }
+    store.checkpoint_states.set_value(target, base_state);
+  }
+}
+
+method update_latest_messages(store: Store, attesting_indices: seq<ValidatorIndex>, attestation: Attestation)
+modifies store.latest_messages
+ensures store.toPure() == update_latest_messages_pure(old(store.toPure()), attesting_indices, attestation)
+{
+  var target: Checkpoint := attestation.data.target;
+  var beacon_block_root: Root := attestation.data.beacon_block_root;
+  var non_equivocating_attesting_indices: seq<ValidatorIndex> := seq_filter_h((i) reads store, store.equivocating_indices => !store.equivocating_indices.contains(i), attesting_indices);
+  var tmp := store.equivocating_indices.repr;
+  assume non_equivocating_attesting_indices == seq_filter((i) => i !in tmp, attesting_indices);
+  var tmp_for_0: seq<ValidatorIndex> := non_equivocating_attesting_indices;
+  
+  ghost var processed: seq<ValidatorIndex> := [];
+  ghost var loop_body := (store: Store_dt, i: ValidatorIndex) =>
+    if i !in store.latest_messages || target.epoch > store.latest_messages[i].epoch then
+      store.(latest_messages := store.latest_messages[i := LatestMessage(target.epoch, beacon_block_root)])
+    else
+      store;
+  while tmp_for_0 != [] decreases tmp_for_0
+  invariant processed + tmp_for_0 == non_equivocating_attesting_indices
+  invariant seq_loop(processed, old(store.toPure()), loop_body) == store.toPure()
+  {
+    var i: ValidatorIndex := tmp_for_0[0];
+    tmp_for_0 := tmp_for_0[1..];
+    if !store.latest_messages.contains(i) || target.epoch > store.latest_messages.get_nf(i).epoch {
+      store.latest_messages.set_value(i, LatestMessage(target.epoch, beacon_block_root));
+    }
+    processed := processed + [i];
+  }
+  assert processed == non_equivocating_attesting_indices;
+}
+
+method on_tick(store: Store, time: uint64)
+returns (status_: Outcome<()>) 
+requires time >= store.time
+requires valid_constants()
+requires valid_time_slots(store)
+requires valid_blocks(store.blocks)
+modifies store
+ensures !status_.IsFailure() <==> !on_tick_pure(old(store.toPure()), time).IsFailure()
+ensures !status_.IsFailure() ==> store.toPure() == on_tick_pure(old(store.toPure()), time).Extract()
+{
+  status_ := Result(());
+  var previous_slot: Slot := get_current_slot(store);
+  store.time := time;
+  var current_slot: Slot := get_current_slot(store);
+  if current_slot > previous_slot {
+    store.proposer_boost_root := Root_new(0);
+  }
+  if !(current_slot > previous_slot && compute_slots_since_epoch_start(current_slot) == 0) {
+    return;
+  }
+  if store.best_justified_checkpoint.epoch > store.justified_checkpoint.epoch {
+    var finalized_slot: Slot := compute_start_slot_at_epoch(store.finalized_checkpoint.epoch);
+    var ancestor_at_finalized_slot :- get_ancestor(store, store.best_justified_checkpoint.root, finalized_slot);
+    if ancestor_at_finalized_slot == store.finalized_checkpoint.root {
+      store.justified_checkpoint := store.best_justified_checkpoint;
+    }
+  }
+}
+
+method on_block(store: Store, signed_block: SignedBeaconBlock)
+returns (status_: Outcome<()>) 
+requires valid_constants()
+requires valid_time_slots(store)
+requires valid_blocks(store.blocks)
+modifies store, store.blocks, store.block_states
+ensures var pure_out := on_block_pure(old(store.toPure()), signed_block);
+        && !status_.IsFailure() <==> !pure_out.IsFailure()
+        && !status_.IsFailure() ==> store.toPure() == pure_out.Extract()
+{
+  status_ := Result(());
+  var block: BeaconBlock := signed_block.message;
+  var _ :- pyassert(store.block_states.contains(block.parent_root));
+  var tmp_0 :- store.block_states.get(block.parent_root);
+  var pre_state: BeaconState := tmp_0.copy();
+  var _ :- pyassert(get_current_slot(store) >= block.slot);
+  var finalized_slot: Slot := compute_start_slot_at_epoch(store.finalized_checkpoint.epoch);
+  var _ :- pyassert(block.slot > finalized_slot);
+  var tmp_1 :- get_ancestor(store, block.parent_root, finalized_slot);
+  var _ :- pyassert(tmp_1 == store.finalized_checkpoint.root);
+  var state: BeaconState := pre_state.copy();
+  state :- state_transition(state, signed_block, true);
+  store.blocks.set_value(hash_tree_root(block), block);
+  assume valid_blocks(store.blocks);
+  store.block_states.set_value(hash_tree_root(block), state);
+  var time_into_slot: uint64 := (store.time - store.genesis_time) % SECONDS_PER_SLOT;
+  var is_before_attesting_interval: bool := time_into_slot < (SECONDS_PER_SLOT / INTERVALS_PER_SLOT);
+  if get_current_slot(store) == block.slot && is_before_attesting_interval {
+    store.proposer_boost_root := Root_new(hash_tree_root(block));
+  }
+  if state.current_justified_checkpoint.epoch > store.justified_checkpoint.epoch {
+    if state.current_justified_checkpoint.epoch > store.best_justified_checkpoint.epoch {
+      store.best_justified_checkpoint := state.current_justified_checkpoint;
+    }
+    var tmp_2 :- should_update_justified_checkpoint(store, state.current_justified_checkpoint);
+    if tmp_2 {
+      store.justified_checkpoint := state.current_justified_checkpoint;
+    }
+  }
+  if state.finalized_checkpoint.epoch > store.finalized_checkpoint.epoch {
+    store.finalized_checkpoint := state.finalized_checkpoint;
+    store.justified_checkpoint := state.current_justified_checkpoint;
+  }
+}
+
+/*
+    Run ``on_attestation`` upon receiving a new ``attestation`` from either within a block or directly on the wire.
+
+    An ``attestation`` that is asserted as invalid may be valid at a later time,
+    consider scheduling it for later processing in such case.
+    */
+method on_attestation(store: Store, attestation: Attestation, is_from_block: bool)
+returns (status_: Outcome<()>) 
+requires valid_constants()
+requires valid_time_slots(store)
+requires valid_blocks(store.blocks)
+modifies store.latest_messages, store.checkpoint_states
+ensures var pure_out := on_attestation_pure(old(store.toPure()), attestation, is_from_block);
+        && !status_.IsFailure() <==> !pure_out.IsFailure()
+        && !status_.IsFailure() ==> store.toPure() == pure_out.Extract()
+{
+  status_ := Result(());
+  var _ :- validate_on_attestation(store, attestation, is_from_block);
+  var _ :- store_target_checkpoint_state(store, attestation.data.target);
+  var target_state: BeaconState :- store.checkpoint_states.get(attestation.data.target);
+  var indexed_attestation: IndexedAttestation := get_indexed_attestation(target_state, attestation);
+  var _ :- pyassert(is_valid_indexed_attestation(target_state, indexed_attestation));
+  update_latest_messages(store, indexed_attestation.attesting_indices, attestation);
+}
+
+/*
+    Run ``on_attester_slashing`` immediately upon receiving a new ``AttesterSlashing``
+    from either within a block or directly on the wire.
+    */
+method on_attester_slashing(store: Store, attester_slashing: AttesterSlashing)
+returns (status_: Outcome<()>) 
+modifies store.equivocating_indices
+{
+  status_ := Result(());
+  var attestation_1: IndexedAttestation := attester_slashing.attestation_1;
+  var attestation_2: IndexedAttestation := attester_slashing.attestation_2;
+  var _ :- pyassert(is_slashable_attestation_data(attestation_1.data, attestation_2.data));
+  var state: BeaconState :- store.block_states.get(store.justified_checkpoint.root);
+  var _ :- pyassert(is_valid_indexed_attestation(state, attestation_1));
+  var _ :- pyassert(is_valid_indexed_attestation(state, attestation_2));
+  var indices: set<ValidatorIndex> := seq_to_set(attestation_1.attesting_indices) * seq_to_set(attestation_2.attesting_indices);
+  var tmp_for_0: set<ValidatorIndex> := indices;
+  while tmp_for_0 != {} decreases tmp_for_0 {
+    var index: ValidatorIndex :| index in tmp_for_0;
+    tmp_for_0 := tmp_for_0 - {index};
+    store.equivocating_indices.add(index);
+  }
+}
